formic_site_duct/implementations/user_info.program.dfy
@@ -1,0 +1,22 @@
+module DuctSaveUserImpl {
+
+  import opened DB
+  import opened DuctTools
+  import opened DuctSpecs
+
+  class UserInfoPage extends UserInfoSpec {
+
+    constructor () {}
+
+    function Implementation(u: UserInfo): GeneratedEndpointResult
+    {
+        
+    }
+
+    lemma ProveImplementationCorrect(u: UserInfo)
+      requires PreCondition(u)
+      ensures ImplementationCorrect(u)
+    {
+    }
+  }
+}
